Charge!/src/Charge/Tactics/BILogic/BILogicTacs.v
@@ -1,0 +1,185 @@
+Require Import Charge.ModularFunc.Denotation.
+Require Import Charge.ModularFunc.BILogicFunc.
+
+Require Import Charge.Tactics.Base.MirrorCoreTacs.
+
+Require Import MirrorCore.TypesI.
+Require Import MirrorCore.ExprI.
+
+Ltac bilf_emp_type :=
+  match goal with
+    | H1 : bilogicS ?e = Some (bilf_emp ?t) |- _ =>
+      match goal with
+        | _ : ExprDsimul.ExprDenote.funcAs e t = Some _ |- _ => fail 1
+        | _ : ExprDsimul.ExprDenote.exprD' _ _ t e = Some _ |- _ => fail 1
+        | H2 : ExprDsimul.ExprDenote.funcAs e _ = Some _ |- _ =>
+  	  	  let H := fresh "H" in
+	        pose proof (bilf_emp_func_type_eq _ _ H1 H2) as H; repeat clear_eq; subst
+	    | H2 : ExprDsimul.ExprDenote.exprD' _ _ _ e = Some _ |- _ =>
+	      let H := fresh "H" in
+	        pose proof (bilf_emp_type_eq _ _ H1 H2) as H; repeat clear_eq; subst
+	  end
+  end.
+
+Ltac bilf_emp_expr :=
+  match goal with
+    | H1 : bilogicS ?e = Some (bilf_emp ?t), gs : bilogic_ops |- _ =>
+      match goal with
+        |  H2 : gs ?t = Some _ |- _ =>
+	      match goal with
+	        | _ : ExprDsimul.ExprDenote.exprD' _ _ t _ =
+	          Some (fun _ _ => BILogic.empSP) |- _ => fail 1
+	        | _ : ExprDsimul.ExprDenote.funcAs _ t =
+	   		  Some BILogic.empSP |- _ => fail 1
+			| H3 : ExprDsimul.ExprDenote.funcAs e t = Some _ |- _ =>
+		 	  let H := fresh "H" in pose proof(bilf_emp_func_eq _ H2 H1 H3); subst
+			| H3 : ExprDsimul.ExprDenote.exprD' _ _ t e = Some _ |- _ =>
+		  	  let H := fresh "H" in pose proof(bilf_emp_eq _ H2 H1 H3); subst
+		 end
+	  end
+  end.
+
+Ltac bilf_star_type :=
+  match goal with
+    | H1 : bilogicS ?e = Some (bilf_star ?t) |- _ =>
+      match goal with
+        | _ : ExprDsimul.ExprDenote.funcAs e (typ2 t (typ2 t t)) = Some _ |- _ => fail 1
+        | _ : ExprDsimul.ExprDenote.exprD' _ _ (typ2 t (typ2 t t)) e = Some _ |- _ => fail 1
+        | H2 : ExprDsimul.ExprDenote.funcAs e _ = Some _ |- _ =>
+  	  	  let H := fresh "H" in
+	        pose proof (bilf_star_func_type_eq _ _ H1 H2) as H; r_inj H; repeat clear_eq; subst
+	    | H2 : ExprDsimul.ExprDenote.exprD' _ _ _ e = Some _ |- _ =>
+	      let H := fresh "H" in
+	        pose proof (bilf_star_type_eq _ _ H1 H2) as H; r_inj H; repeat clear_eq; subst
+	  end
+  end.
+
+Ltac bilf_star_expr :=
+  match goal with
+    | H1 : bilogicS ?e = Some (bilf_star ?t), gs : bilogic_ops |- _ =>
+      match goal with 
+        | H2 : gs t = Some _ |- _ => 
+	      match goal with
+	        | _ : ExprDsimul.ExprDenote.exprD' _ _ (typ2 t (typ2 t t)) _ =
+	          Some (fun _ _ => starD t _) |- _ => fail 1
+	        | _ : ExprDsimul.ExprDenote.funcAs _ (typ2 t (typ2 t t)) =
+	   		  Some (starD t _) |- _ => fail 1
+			| H3 : ExprDsimul.ExprDenote.funcAs e (typ2 t (typ2 t t)) = Some _ |- _ =>
+		 	  let H := fresh "H" in pose proof(bilf_star_func_eq _ H2 H1 H3); subst
+			| H3 : ExprDsimul.ExprDenote.exprD' _ _ (typ2 t (typ2 t t)) e = Some _ |- _ =>
+		  	  let H := fresh "H" in pose proof(bilf_star_eq _ H2 H1 H3); subst
+		  end
+      end
+  end.
+
+Ltac bilf_wand_type :=
+  match goal with
+    | H1 : bilogicS ?e = Some (bilf_wand ?t) |- _ =>
+      match goal with
+        | _ : ExprDsimul.ExprDenote.funcAs e (typ2 t (typ2 t t)) = Some _ |- _ => fail 1
+        | _ : ExprDsimul.ExprDenote.exprD' _ _ (typ2 t (typ2 t t)) e = Some _ |- _ => fail 1
+        | H2 : ExprDsimul.ExprDenote.funcAs e _ = Some _ |- _ =>
+  	  	  let H := fresh "H" in
+	        pose proof (bilf_wand_func_type_eq _ _ H1 H2) as H; r_inj H; repeat clear_eq; subst
+	    | H2 : ExprDsimul.ExprDenote.exprD' _ _ _ e = Some _ |- _ =>
+	      let H := fresh "H" in
+	        pose proof (bilf_wand_type_eq _ _ H1 H2) as H; r_inj H; repeat clear_eq; subst
+	  end
+  end.
+
+Ltac bilf_wand_expr :=
+  match goal with
+    | H1 : bilogicS ?e = Some (bilf_wand ?t), gs : bilogic_ops |- _ =>
+      match goal with 
+        | H2 : gs t = Some _ |- _ => 
+	      match goal with
+	        | _ : ExprDsimul.ExprDenote.exprD' _ _ (typ2 t (typ2 t t)) _ =
+	          Some (fun _ _ => wandD t _) |- _ => fail 1
+	        | _ : ExprDsimul.ExprDenote.funcAs _ (typ2 t (typ2 t t)) =
+	   		  Some (wandD t _) |- _ => fail 1
+			| H3 : ExprDsimul.ExprDenote.funcAs e (typ2 t (typ2 t t)) = Some _ |- _ =>
+		 	  let H := fresh "H" in pose proof(bilf_wand_func_eq _ H2 H1 H3); subst
+			| H3 : ExprDsimul.ExprDenote.exprD' _ _ (typ2 t (typ2 t t)) e = Some _ |- _ =>
+		  	  let H := fresh "H" in pose proof(bilf_wand_eq _ H2 H1 H3); subst
+		  end
+      end
+  end.
+
+
+Ltac bil_pointwise_bilogicD :=  
+  match goal with
+    | bilp : bil_pointwise, gs : bilogic_ops |- _ =>
+      match goal with
+        | H1 : bilp (typ2 ?t ?u) = true |- _ =>
+          match goal with
+            | _ : gs (typ2 t u) = Some _ |- _ => fail 1
+            | H2 : bil_pointwiseOk gs bilp |- _ => destruct (bil_pointwise_bilogic H2 _ _ H1)
+          end
+      end
+  end.
+
+Ltac bil_pointwise_bilogic_rangeD :=  
+  match goal with
+    | bilp : bil_pointwise, gs : bilogic_ops |- _ =>
+      match goal with
+        | H1 : bilp (typ2 ?t ?u) = true |- _ =>
+          match goal with
+            | _ : gs u = Some _ |- _ => fail 1
+            | H2 : bil_pointwiseOk gs bilp |- _ => destruct (bil_pointwise_bilogic_range H2 _ _ H1)
+          end
+      end
+  end.
+
+Ltac bilf_unfold := 
+  first [
+    progress (unfold empD) |
+    progress (unfold starD) |
+    progress (unfold wandD)
+  ].
+
+Ltac pointwise_empD_rewrite :=
+  match goal with
+    | gs : bilogic_ops, bilp : bil_pointwise |- context [trmD BILogic.empSP _ _] =>
+      match goal with
+        | H1 : bil_pointwiseOk gs bilp, H2 : bilp (typ2 ?t ?u) = true,
+          H3 : gs (typ2 ?t ?u) = Some _, H4 : gs ?u = Some _ |- _ =>
+     	  let H := fresh "H" in 
+     	    pose proof (bil_pointwise_empD H1 _ _ H2 H3 H4) as H;
+     	    unfold tyArrD, tyArrD' in H; simpl in H; simpl; rewriteD H; clear H
+      end
+  end.
+
+Ltac pointwise_empR_rewrite :=
+  match goal with
+    | gs : bilogic_ops, bilp : bil_pointwise |- context [trmR (fun x : _ => BILogic.empSP) _] =>
+      match goal with
+        | H1 : bil_pointwiseOk gs bilp, H2 : bilp (typ2 ?t ?u) = true,
+          H3 : gs (typ2 ?t ?u) = Some _, H4 : gs ?u = Some _ |- _ =>
+     	  let H := fresh "H" in 
+     	    pose proof (bil_pointwise_empR H1 _ _ H2 H3 H4) as H;
+     	    unfold tyArrR, tyArrR' in H; simpl in H; simpl; rewriteD H; clear H
+      end
+  end.
+
+Ltac bilf_rewrite := 
+  first [
+    pointwise_empD_rewrite |
+    pointwise_empR_rewrite
+  ].
+
+Ltac bilf_forward_step :=
+  match goal with 
+    | H : Some _ = bilogicS _ |- _ =>  symmetry in H
+    | _ => 
+       first [
+        bil_pointwise_bilogicD |
+        bil_pointwise_bilogic_rangeD |
+        bilf_emp_type |
+        bilf_star_type |
+        bilf_wand_type |
+        bilf_emp_expr |
+        bilf_star_expr |
+        bilf_wand_expr
+        
+      ]
+  end.
