Charge!/src/Charge/Tactics/ILEmbed/ILEmbedTacs.v
@@ -1,0 +1,49 @@
+Require Import Charge.ModularFunc.EmbedFunc.
+
+Require Import Charge.Tactics.Base.MirrorCoreTacs.
+
+Require Import MirrorCore.TypesI.
+Require Import MirrorCore.ExprI.
+
+Ltac eilf_embed_type :=
+  match goal with
+    | H1 : embedS ?e = Some (eilf_embed ?t ?u) |- _ =>
+      match goal with
+        | _ : ExprDsimul.ExprDenote.funcAs e (typ2 t u) = Some _ |- _ => fail 1
+        | _ : ExprDsimul.ExprDenote.exprD' _ _ (typ2 t u) e = Some _ |- _ => fail 1
+        | H2 : ExprDsimul.ExprDenote.funcAs e _ = Some _ |- _ =>
+  	  	  let H := fresh "H" in
+	        pose proof (eilf_embed_func_type_eq _ _ H1 H2) as H; r_inj H; repeat clear_eq; subst
+	    | H2 : ExprDsimul.ExprDenote.exprD' _ _ _ e = Some _ |- _ =>
+	      let H := fresh "H" in
+	        pose proof (eilf_embed_type_eq _ _ H1 H2) as H; r_inj H; repeat clear_eq; subst
+	  end
+  end.
+
+Ltac eilf_embed_expr :=
+  match goal with
+    | H1 : embedS ?e = Some (eilf_embed ?t ?u), gs : embed_ops |- _ =>
+      match goal with 
+        | H2 : gs t u = Some _ |- _ => 
+	      match goal with
+	        | _ : ExprDsimul.ExprDenote.exprD' _ _ (typ2 t u) _ =
+	          Some (fun _ _ => embedD t u _) |- _ => fail 1
+	        | _ : ExprDsimul.ExprDenote.funcAs _ (typ2 t u) =
+	   		  Some (embedD t u _) |- _ => fail 1
+			| H3 : ExprDsimul.ExprDenote.funcAs e (typ2 t u) = Some _ |- _ =>
+		 	  let H := fresh "H" in pose proof(eilf_embed_func_eq _ H2 H1 H3); subst
+			| H3 : ExprDsimul.ExprDenote.exprD' _ _ (typ2 t u) e = Some _ |- _ =>
+		  	  let H := fresh "H" in pose proof(eilf_embed_eq _ H2 H1 H3); subst
+		  end
+      end
+  end.
+  
+Ltac eilf_forward_step :=
+  match goal with 
+    | H : Some _ = embedS _ |- _ =>  symmetry in H
+    | _ => 
+       first [
+        eilf_embed_type |
+        eilf_embed_expr
+      ]
+  end.
