Charge!/src/Charge/Tactics/Open/OpenTacs.v
@@ -74,16 +74,149 @@ Ltac of_const_expr :=
 	  	  let H := fresh "H" in pose proof(of_const_eq _ H1 H2); subst
 	 end
   end.
+  
+Ltac of_ap_type :=
+  match goal with
+    | H1 : open_funcS ?e = Some (of_ap ?t ?u) |- _ =>
+      match goal with
+        | _ : ExprDsimul.ExprDenote.funcAs e
+   			  (typ2 (typ2 tyStack (typ2 t u))
+                (typ2 (typ2 tyStack t) (typ2 tyStack u))) = Some _ |- _ => fail 1
+        | _ : ExprDsimul.ExprDenote.exprD' _ _  
+              (typ2 (typ2 tyStack (typ2 t u))
+                (typ2 (typ2 tyStack t) (typ2 tyStack u))) e = Some _ |- _ => fail 1
+        | H2 : ExprDsimul.ExprDenote.funcAs e _ = Some _ |- _ =>
+  	  	  let H := fresh "H" in
+	        pose proof (of_ap_func_type_eq _ _ H1 H2) as H; r_inj H; repeat clear_eq; subst
+	    | H2 : ExprDsimul.ExprDenote.exprD' _ _ _ e = Some _ |- _ =>
+	      let H := fresh "H" in
+	        pose proof (of_ap_type_eq _ _ H1 H2) as H; r_inj H; repeat clear_eq; subst
+	  end
+  end.
 
-Ltac of_forward_step :=
+Ltac of_ap_expr :=
+  match goal with
+    | H1 : open_funcS ?e = Some (of_ap ?t ?u) |- _ =>
+      match goal with
+        | _ : ExprDsimul.ExprDenote.exprD' _ _ 
+              (typ2 (typ2 tyStack (typ2 t u))
+                (typ2 (typ2 tyStack t) (typ2 tyStack u))) e =
+          Some (fun _ _ => apD t u) |- _ => fail 1
+        | _ : ExprDsimul.ExprDenote.funcAs e 
+  			  (typ2 (typ2 tyStack (typ2 t u))
+                (typ2 (typ2 tyStack t) (typ2 tyStack u))) =
+   		  Some (apD t u) |- _ => fail 1
+		| H2 : ExprDsimul.ExprDenote.funcAs e 
+			   (typ2 (typ2 tyStack (typ2 t u))
+                (typ2 (typ2 tyStack t) (typ2 tyStack u))) = Some _ |- _ =>
+	 	  let H := fresh "H" in pose proof(of_ap_func_eq _ H1 H2); subst
+		| H2 : ExprDsimul.ExprDenote.exprD' _ _ 
+			   (typ2 (typ2 tyStack (typ2 t u))
+                (typ2 (typ2 tyStack t) (typ2 tyStack u))) e = Some _ |- _ =>
+	  	  let H := fresh "H" in pose proof(of_ap_eq _ H1 H2); subst
+	 end
+  end.
+
+Ltac of_trunc_subst_type :=
+  match goal with
+    | H1 : open_funcS ?e = Some of_trunc_subst |- _ =>
+      match goal with
+        | _ : ExprDsimul.ExprDenote.funcAs e
+   			  (typ2 (tyList (tyProd tyString tyExpr)) (typ2 tyString tyExpr)) = Some _ |- _ => fail 1
+        | _ : ExprDsimul.ExprDenote.exprD' _ _  
+              (typ2 (tyList (tyProd tyString tyExpr)) (typ2 tyString tyExpr)) e = Some _ |- _ => fail 1
+        | H2 : ExprDsimul.ExprDenote.funcAs e _ = Some _ |- _ =>
+  	  	  let H := fresh "H" in
+	        pose proof (of_trunc_subst_func_type_eq _ _ H1 H2) as H; r_inj H; repeat clear_eq; subst
+        | H2 : ExprDsimul.ExprDenote.exprD' _ _ _ _ e = Some _ |- _ =>
+  	  	  let H := fresh "H" in
+	        pose proof (of_trunc_subst_type_eq _ _ H1 H2) as H; r_inj H; repeat clear_eq; subst
+	  end
+  end.
+
+Ltac of_trunc_subst_expr :=
+  match goal with
+    | H1 : open_funcS ?e = Some of_trunc_subst |- _ =>
+      match goal with
+        | _ : ExprDsimul.ExprDenote.exprD' _ _ 
+              (typ2 (tyList (tyProd tyString tyExpr)) (typ2 tyString tyExpr)) e =
+          Some (fun _ _ => truncSubstD) |- _ => fail 1
+        | _ : ExprDsimul.ExprDenote.funcAs e 
+  			  (typ2 (tyList (tyProd tyString tyExpr)) (typ2 tyString tyExpr)) =
+   		  Some truncSubstD |- _ => fail 1
+		| H2 : ExprDsimul.ExprDenote.funcAs e 
+			   (typ2 (tyList (tyProd tyString tyExpr)) (typ2 tyString tyExpr)) = Some _ |- _ =>
+	 	  let H := fresh "H" in pose proof(of_trunc_subst_func_eq _ H1 H2); subst
+		| H2 : ExprDsimul.ExprDenote.exprD' _ _ 
+			   (typ2 tyString (typ2 tyStack tyVal)) e = Some _ |- _ =>
+	  	  let H := fresh "H" in pose proof(of_trunc_subst_eq _ H1 H2); subst
+	 end
+  end.
+
+Ltac of_stack_get_type :=
+  match goal with
+    | H1 : open_funcS ?e = Some of_stack_get |- _ =>
+      match goal with
+        | _ : ExprDsimul.ExprDenote.funcAs e
+   			  (typ2 tyString (typ2 (typ2 tyString tyVal) tyVal)) = Some _ |- _ => fail 1
+        | _ : ExprDsimul.ExprDenote.exprD' _ _  
+              (typ2 tyString (typ2 (typ2 tyString tyVal) tyVal)) e = Some _ |- _ => fail 1
+        | H2 : ExprDsimul.ExprDenote.funcAs e _ = Some _ |- _ =>
+  	  	  let H := fresh "H" in
+	        pose proof (of_stack_get_func_type_eq _ _ H1 H2) as H; r_inj H; repeat clear_eq; subst
+        | H2 : ExprDsimul.ExprDenote.exprD' _ _ _ _ e = Some _ |- _ =>
+  	  	  let H := fresh "H" in
+	        pose proof (of_stack_get_type_eq _ _ H1 H2) as H; r_inj H; repeat clear_eq; subst
+	  end
+  end.
+
+Ltac of_stack_get_expr :=
+  match goal with
+    | H1 : open_funcS ?e = Some of_stack_get |- _ =>
+      match goal with
+        | _ : ExprDsimul.ExprDenote.exprD' _ _ 
+              (typ2 tyString (typ2 (typ2 tyString tyVal) tyVal)) e =
+          Some (fun _ _ => stack_getD) |- _ => fail 1
+        | _ : ExprDsimul.ExprDenote.funcAs e 
+  			  (typ2 tyString (typ2 (typ2 tyString tyVal) tyVal)) =
+   		  Some stack_getD |- _ => fail 1
+		| H2 : ExprDsimul.ExprDenote.funcAs e 
+			   (typ2 tyString (typ2 (typ2 tyString tyVal) tyVal)) = Some _ |- _ =>
+	 	  let H := fresh "H" in pose proof(of_stack_get_func_eq _ H1 H2); subst
+		| H2 : ExprDsimul.ExprDenote.exprD' _ _ 
+			   (typ2 tyString (typ2 (typ2 tyString tyVal) tyVal)) e = Some _ |- _ =>
+	  	  let H := fresh "H" in pose proof(of_stack_get_eq _ H1 H2); subst
+	 end
+  end.
+
+Ltac of_unfold := 
+  first [
+    progress (unfold applySubstD) |
+    progress (unfold constD) |
+    progress (unfold apD) | 
+    progress (unfold truncSubstD) | 
+    progress (unfold parSubstD) |
+    progress (unfold stack_getD) |
+    progress (unfold substD) |
+    progress (unfold substR) |
+    progress (unfold substListD)
+  ].
+  
+  Ltac of_forward_step :=
   match goal with 
     | H : Some _ = open_funcS _ |- _ =>  symmetry in H
     | _ => 
        first [
         of_apply_subst_type |
         of_const_type |
+        of_ap_type |
+        of_trunc_subst_type |
+        of_stack_get_type |
         of_apply_subst_expr |
-        of_const_expr
+        of_const_expr |
+        of_ap_expr |
+        of_trunc_subst_expr |
+        of_stack_get_expr
       ]
   end.
     
