Charge!/src/Charge/Tactics/Open/Subst.v
@@ -44,7 +44,7 @@ Section ApplySubst.
 		    	
 	Fixpoint applyTruncSubst (t : typ) (x : String.string) (lst : expr typ func) : expr typ func :=
 	  match listS lst with
-	    | Some (pNil u) => mkNull
+	    | Some (pNil u) => mkConst tyVal mkNull
 	    | _ => 
 	      match lst with
 	        | App (App f (App (App g y) e)) ys =>
@@ -404,366 +404,9 @@ Require Import Charge.Tactics.Base.DenotationTacs.
 Require Import Charge.Tactics.Base.MirrorCoreTacs.
 Require Import MirrorCore.Lambda.Expr.
 
-Ltac ilf_true_type :=
-  match goal with
-    | H1 : ilogicS ?e = Some (ilf_true ?t) |- _ =>
-      match goal with
-        | _ : ExprDsimul.ExprDenote.funcAs e t = Some _ |- _ => fail 1
-        | _ : ExprDsimul.ExprDenote.exprD' _ _ t e = Some _ |- _ => fail 1
-        | H2 : ExprDsimul.ExprDenote.funcAs e _ = Some _ |- _ =>
-  	  	  let H := fresh "H" in
-	        pose proof (ilf_true_func_type_eq _ _ H1 H2) as H; repeat clear_eq; subst
-	    | H2 : ExprDsimul.ExprDenote.exprD' _ _ _ e = Some _ |- _ =>
-	      let H := fresh "H" in
-	        pose proof (ilf_true_type_eq _ _ H1 H2) as H; repeat clear_eq; subst
-	  end
-  end.
+Print Typ2.
+Print Typ2Ok.
 
-Ltac ilf_true_expr :=
-  match goal with
-    | H1 : ilogicS ?e = Some (ilf_true ?t), gs : logic_ops, H2 : gs ?t = Some _ |- _ =>
-      match goal with
-        | _ : ExprDsimul.ExprDenote.exprD' _ _ t _ =
-          Some (fun _ _ => trueD _ H2) |- _ => fail 1
-        | _ : ExprDsimul.ExprDenote.funcAs _ t =
-   		  Some (trueD _ H2) |- _ => fail 1
-		| H3 : ExprDsimul.ExprDenote.funcAs e t = Some _ |- _ =>
-	 	  let H := fresh "H" in pose proof(ilf_true_func_eq _ H2 H1 H3); subst
-		| H3 : ExprDsimul.ExprDenote.exprD' _ _ t e = Some _ |- _ =>
-	  	  let H := fresh "H" in pose proof(ilf_true_eq _ H2 H1 H3); subst
-	 end
-  end.
-
-Ltac ilf_false_type :=
-  match goal with
-    | H1 : ilogicS ?e = Some (ilf_false ?t) |- _ =>
-      match goal with
-        | _ : ExprDsimul.ExprDenote.funcAs e t = Some _ |- _ => fail 1
-        | _ : ExprDsimul.ExprDenote.exprD' _ _ t e = Some _ |- _ => fail 1
-        | H2 : ExprDsimul.ExprDenote.funcAs e _ = Some _ |- _ =>
-  	  	  let H := fresh "H" in
-	        pose proof (ilf_false_func_type_eq _ _ H1 H2) as H; repeat clear_eq; subst
-	    | H2 : ExprDsimul.ExprDenote.exprD' _ _ _ e = Some _ |- _ =>
-	      let H := fresh "H" in
-	        pose proof (ilf_false_type_eq _ _ H1 H2) as H; repeat clear_eq; subst
-	  end
-  end.
-
-Ltac ilf_false_expr :=
-  match goal with
-    | H1 : ilogicS ?e = Some (ilf_false ?t), gs : logic_ops, H2 : gs ?t = Some _ |- _ =>
-      match goal with
-        | _ : ExprDsimul.ExprDenote.exprD' _ _ t _ =
-          Some (fun _ _ => falseD _ H2) |- _ => fail 1
-        | _ : ExprDsimul.ExprDenote.funcAs _ t =
-   		  Some (falseD _ H2) |- _ => fail 1
-		| H3 : ExprDsimul.ExprDenote.funcAs e t = Some _ |- _ =>
-	 	  let H := fresh "H" in pose proof(ilf_false_func_eq _ H2 H1 H3); subst
-		| H3 : ExprDsimul.ExprDenote.exprD' _ _ t e = Some _ |- _ =>
-	  	  let H := fresh "H" in pose proof(ilf_false_eq _ H2 H1 H3); subst
-	 end
-  end.
-
-Ltac ilf_and_type :=
-  match goal with
-    | H1 : ilogicS ?e = Some (ilf_and ?t) |- _ =>
-      match goal with
-        | _ : ExprDsimul.ExprDenote.funcAs e (typ2 t (typ2 t t)) = Some _ |- _ => fail 1
-        | _ : ExprDsimul.ExprDenote.exprD' _ _ (typ2 t (typ2 t t)) e = Some _ |- _ => fail 1
-        | H2 : ExprDsimul.ExprDenote.funcAs e _ = Some _ |- _ =>
-  	  	  let H := fresh "H" in
-	        pose proof (ilf_and_func_type_eq _ _ H1 H2) as H; r_inj H; repeat clear_eq; subst
-	    | H2 : ExprDsimul.ExprDenote.exprD' _ _ _ e = Some _ |- _ =>
-	      let H := fresh "H" in
-	        pose proof (ilf_and_type_eq _ _ H1 H2) as H; r_inj H; repeat clear_eq; subst
-	  end
-  end.
-
-Ltac ilf_and_expr :=
-  match goal with
-    | H1 : ilogicS ?e = Some (ilf_and ?t), gs : logic_ops, H2 : gs ?t = Some _ |- _ =>
-      match goal with
-        | _ : ExprDsimul.ExprDenote.exprD' _ _ (typ2 t (typ2 t t)) _ =
-          Some (fun _ _ => andD _ H2) |- _ => fail 1
-        | _ : ExprDsimul.ExprDenote.funcAs _ (typ2 t (typ2 t t)) =
-   		  Some (andD _ H2) |- _ => fail 1
-		| H3 : ExprDsimul.ExprDenote.funcAs e (typ2 t (typ2 t t)) = Some _ |- _ =>
-	 	  let H := fresh "H" in pose proof(ilf_and_func_eq _ H2 H1 H3); subst
-		| H3 : ExprDsimul.ExprDenote.exprD' _ _ (typ2 t (typ2 t t)) e = Some _ |- _ =>
-	  	  let H := fresh "H" in pose proof(ilf_and_eq _ H2 H1 H3); subst
-	 end
-  end.
-
-Ltac ilf_or_type :=
-  match goal with
-    | H1 : ilogicS ?e = Some (ilf_or ?t) |- _ =>
-      match goal with
-        | _ : ExprDsimul.ExprDenote.funcAs e (typ2 t (typ2 t t)) = Some _ |- _ => fail 1
-        | _ : ExprDsimul.ExprDenote.exprD' _ _ (typ2 t (typ2 t t)) e = Some _ |- _ => fail 1
-        | H2 : ExprDsimul.ExprDenote.funcAs e _ = Some _ |- _ =>
-  	  	  let H := fresh "H" in
-	        pose proof (ilf_or_func_type_eq _ _ H1 H2) as H; r_inj H; repeat clear_eq; subst
-	    | H2 : ExprDsimul.ExprDenote.exprD' _ _ _ e = Some _ |- _ =>
-	      let H := fresh "H" in
-	        pose proof (ilf_or_type_eq _ _ H1 H2) as H; r_inj H; repeat clear_eq; subst
-	  end
-  end.
-
-Ltac ilf_or_expr :=
-  match goal with
-    | H1 : ilogicS ?e = Some (ilf_or ?t), gs : logic_ops, H2 : gs ?t = Some _ |- _ =>
-      match goal with
-        | _ : ExprDsimul.ExprDenote.exprD' _ _ (typ2 t (typ2 t t)) _ =
-          Some (fun _ _ => orD _ H2) |- _ => fail 1
-        | _ : ExprDsimul.ExprDenote.funcAs _ (typ2 t (typ2 t t)) =
-   		  Some (orD _ H2) |- _ => fail 1
-		| H3 : ExprDsimul.ExprDenote.funcAs e (typ2 t (typ2 t t)) = Some _ |- _ =>
-	 	  let H := fresh "H" in pose proof(ilf_or_func_eq _ H2 H1 H3); subst
-		| H3 : ExprDsimul.ExprDenote.exprD' _ _ (typ2 t (typ2 t t)) e = Some _ |- _ =>
-	  	  let H := fresh "H" in pose proof(ilf_or_eq _ H2 H1 H3); subst
-	 end
-  end.
-
-Ltac ilf_impl_type :=
-  match goal with
-    | H1 : ilogicS ?e = Some (ilf_impl ?t) |- _ =>
-      match goal with
-        | _ : ExprDsimul.ExprDenote.funcAs e (typ2 t (typ2 t t)) = Some _ |- _ => fail 1
-        | _ : ExprDsimul.ExprDenote.exprD' _ _ (typ2 t (typ2 t t)) e = Some _ |- _ => fail 1
-        | H2 : ExprDsimul.ExprDenote.funcAs e _ = Some _ |- _ =>
-  	  	  let H := fresh "H" in
-	        pose proof (ilf_impl_func_type_eq _ _ H1 H2) as H; r_inj H; repeat clear_eq; subst
-	    | H2 : ExprDsimul.ExprDenote.exprD' _ _ _ e = Some _ |- _ =>
-	      let H := fresh "H" in
-	        pose proof (ilf_impl_type_eq _ _ H1 H2) as H; r_inj H; repeat clear_eq; subst
-	  end
-  end.
-
-Ltac ilf_impl_expr :=
-  match goal with
-    | H1 : ilogicS ?e = Some (ilf_impl ?t), gs : logic_ops, H2 : gs ?t = Some _ |- _ =>
-      match goal with
-        | _ : ExprDsimul.ExprDenote.exprD' _ _ (typ2 t (typ2 t t)) _ =
-          Some (fun _ _ => implD _ H2) |- _ => fail 1
-        | _ : ExprDsimul.ExprDenote.funcAs _ (typ2 t (typ2 t t)) =
-   		  Some (implD _ H2) |- _ => fail 1
-		| H3 : ExprDsimul.ExprDenote.funcAs e (typ2 t (typ2 t t)) = Some _ |- _ =>
-	 	  let H := fresh "H" in pose proof(ilf_impl_func_eq _ H2 H1 H3); subst
-		| H3 : ExprDsimul.ExprDenote.exprD' _ _ (typ2 t (typ2 t t)) e = Some _ |- _ =>
-	  	  let H := fresh "H" in pose proof(ilf_impl_eq _ H2 H1 H3); subst
-	 end
-  end.
-  
-Ltac bilf_emp_type :=
-  match goal with
-    | H1 : bilogicS ?e = Some (bilf_emp ?t) |- _ =>
-      match goal with
-        | _ : ExprDsimul.ExprDenote.funcAs e t = Some _ |- _ => fail 1
-        | _ : ExprDsimul.ExprDenote.exprD' _ _ t e = Some _ |- _ => fail 1
-        | H2 : ExprDsimul.ExprDenote.funcAs e _ = Some _ |- _ =>
-  	  	  let H := fresh "H" in
-	        pose proof (bilf_emp_func_type_eq _ _ H1 H2) as H; repeat clear_eq; subst
-	    | H2 : ExprDsimul.ExprDenote.exprD' _ _ _ e = Some _ |- _ =>
-	      let H := fresh "H" in
-	        pose proof (bilf_emp_type_eq _ _ H1 H2) as H; repeat clear_eq; subst
-	  end
-  end.
-
-Ltac bilf_emp_expr :=
-  match goal with
-    | H1 : bilogicS ?e = Some (bilf_emp ?t), gs : bilogic_ops |- _ =>
-      match goal with
-        |  H2 : gs ?t = Some _ |- _ =>
-	      match goal with
-	        | _ : ExprDsimul.ExprDenote.exprD' _ _ t _ =
-	          Some (fun _ _ => empD t _) |- _ => fail 1
-	        | _ : ExprDsimul.ExprDenote.funcAs _ t =
-	   		  Some (empD t _) |- _ => fail 1
-			| H3 : ExprDsimul.ExprDenote.funcAs e t = Some _ |- _ =>
-		 	  let H := fresh "H" in pose proof(bilf_emp_func_eq _ H2 H1 H3); subst
-			| H3 : ExprDsimul.ExprDenote.exprD' _ _ t e = Some _ |- _ =>
-		  	  let H := fresh "H" in pose proof(bilf_emp_eq _ H2 H1 H3); subst
-		 end
-	  end
-  end.
-
-Ltac bilf_star_type :=
-  match goal with
-    | H1 : bilogicS ?e = Some (bilf_star ?t) |- _ =>
-      match goal with
-        | _ : ExprDsimul.ExprDenote.funcAs e (typ2 t (typ2 t t)) = Some _ |- _ => fail 1
-        | _ : ExprDsimul.ExprDenote.exprD' _ _ (typ2 t (typ2 t t)) e = Some _ |- _ => fail 1
-        | H2 : ExprDsimul.ExprDenote.funcAs e _ = Some _ |- _ =>
-  	  	  let H := fresh "H" in
-	        pose proof (bilf_star_func_type_eq _ _ H1 H2) as H; r_inj H; repeat clear_eq; subst
-	    | H2 : ExprDsimul.ExprDenote.exprD' _ _ _ e = Some _ |- _ =>
-	      let H := fresh "H" in
-	        pose proof (bilf_star_type_eq _ _ H1 H2) as H; r_inj H; repeat clear_eq; subst
-	  end
-  end.
-
-Ltac bilf_star_expr :=
-  match goal with
-    | H1 : bilogicS ?e = Some (bilf_star ?t), gs : bilogic_ops |- _ =>
-      match goal with 
-        | H2 : gs t = Some _ |- _ => 
-	      match goal with
-	        | _ : ExprDsimul.ExprDenote.exprD' _ _ (typ2 t (typ2 t t)) _ =
-	          Some (fun _ _ => starD t _) |- _ => fail 1
-	        | _ : ExprDsimul.ExprDenote.funcAs _ (typ2 t (typ2 t t)) =
-	   		  Some (starD t _) |- _ => fail 1
-			| H3 : ExprDsimul.ExprDenote.funcAs e (typ2 t (typ2 t t)) = Some _ |- _ =>
-		 	  let H := fresh "H" in pose proof(bilf_star_func_eq _ H2 H1 H3); subst
-			| H3 : ExprDsimul.ExprDenote.exprD' _ _ (typ2 t (typ2 t t)) e = Some _ |- _ =>
-		  	  let H := fresh "H" in pose proof(bilf_star_eq _ H2 H1 H3); subst
-		  end
-      end
-  end.
-
-Ltac bilf_wand_type :=
-  match goal with
-    | H1 : bilogicS ?e = Some (bilf_wand ?t) |- _ =>
-      match goal with
-        | _ : ExprDsimul.ExprDenote.funcAs e (typ2 t (typ2 t t)) = Some _ |- _ => fail 1
-        | _ : ExprDsimul.ExprDenote.exprD' _ _ (typ2 t (typ2 t t)) e = Some _ |- _ => fail 1
-        | H2 : ExprDsimul.ExprDenote.funcAs e _ = Some _ |- _ =>
-  	  	  let H := fresh "H" in
-	        pose proof (bilf_wand_func_type_eq _ _ H1 H2) as H; r_inj H; repeat clear_eq; subst
-	    | H2 : ExprDsimul.ExprDenote.exprD' _ _ _ e = Some _ |- _ =>
-	      let H := fresh "H" in
-	        pose proof (bilf_wand_type_eq _ _ H1 H2) as H; r_inj H; repeat clear_eq; subst
-	  end
-  end.
-
-Ltac bilf_wand_expr :=
-  match goal with
-    | H1 : bilogicS ?e = Some (bilf_wand ?t), gs : bilogic_ops |- _ =>
-      match goal with 
-        | H2 : gs t = Some _ |- _ => 
-	      match goal with
-	        | _ : ExprDsimul.ExprDenote.exprD' _ _ (typ2 t (typ2 t t)) _ =
-	          Some (fun _ _ => wandD t _) |- _ => fail 1
-	        | _ : ExprDsimul.ExprDenote.funcAs _ (typ2 t (typ2 t t)) =
-	   		  Some (wandD t _) |- _ => fail 1
-			| H3 : ExprDsimul.ExprDenote.funcAs e (typ2 t (typ2 t t)) = Some _ |- _ =>
-		 	  let H := fresh "H" in pose proof(bilf_wand_func_eq _ H2 H1 H3); subst
-			| H3 : ExprDsimul.ExprDenote.exprD' _ _ (typ2 t (typ2 t t)) e = Some _ |- _ =>
-		  	  let H := fresh "H" in pose proof(bilf_wand_eq _ H2 H1 H3); subst
-		  end
-      end
-  end.
-
-Ltac eilf_embed_type :=
-  match goal with
-    | H1 : embedS ?e = Some (eilf_embed ?t ?u) |- _ =>
-      match goal with
-        | _ : ExprDsimul.ExprDenote.funcAs e (typ2 t u) = Some _ |- _ => fail 1
-        | _ : ExprDsimul.ExprDenote.exprD' _ _ (typ2 t u) e = Some _ |- _ => fail 1
-        | H2 : ExprDsimul.ExprDenote.funcAs e _ = Some _ |- _ =>
-  	  	  let H := fresh "H" in
-	        pose proof (eilf_embed_func_type_eq _ _ H1 H2) as H; r_inj H; repeat clear_eq; subst
-	    | H2 : ExprDsimul.ExprDenote.exprD' _ _ _ e = Some _ |- _ =>
-	      let H := fresh "H" in
-	        pose proof (eilf_embed_type_eq _ _ H1 H2) as H; r_inj H; repeat clear_eq; subst
-	  end
-  end.
-
-Ltac eilf_embed_expr :=
-  match goal with
-    | H1 : embedS ?e = Some (eilf_embed ?t ?u), gs : embed_ops |- _ =>
-      match goal with 
-        | H2 : gs t u = Some _ |- _ => 
-	      match goal with
-	        | _ : ExprDsimul.ExprDenote.exprD' _ _ (typ2 t u) _ =
-	          Some (fun _ _ => embedD t u _) |- _ => fail 1
-	        | _ : ExprDsimul.ExprDenote.funcAs _ (typ2 t u) =
-	   		  Some (embedD t u _) |- _ => fail 1
-			| H3 : ExprDsimul.ExprDenote.funcAs e (typ2 t u) = Some _ |- _ =>
-		 	  let H := fresh "H" in pose proof(eilf_embed_func_eq _ H2 H1 H3); subst
-			| H3 : ExprDsimul.ExprDenote.exprD' _ _ (typ2 t u) e = Some _ |- _ =>
-		  	  let H := fresh "H" in pose proof(eilf_embed_eq _ H2 H1 H3); subst
-		  end
-      end
-  end.
-
-
-Ltac of_ap_type :=
-  match goal with
-    | H1 : open_funcS ?e = Some (of_ap ?t ?u) |- _ =>
-      match goal with
-        | _ : ExprDsimul.ExprDenote.funcAs e
-   			  (typ2 (typ2 tyStack (typ2 t u))
-                (typ2 (typ2 tyStack t) (typ2 tyStack u))) = Some _ |- _ => fail 1
-        | _ : ExprDsimul.ExprDenote.exprD' _ _  
-              (typ2 (typ2 tyStack (typ2 t u))
-                (typ2 (typ2 tyStack t) (typ2 tyStack u))) e = Some _ |- _ => fail 1
-        | H2 : ExprDsimul.ExprDenote.funcAs e _ = Some _ |- _ =>
-  	  	  let H := fresh "H" in
-	        pose proof (of_ap_func_type_eq _ _ H1 H2) as H; r_inj H; repeat clear_eq; subst
-	    | H2 : ExprDsimul.ExprDenote.exprD' _ _ _ e = Some _ |- _ =>
-	      let H := fresh "H" in
-	        pose proof (of_ap_type_eq _ _ H1 H2) as H; r_inj H; repeat clear_eq; subst
-	  end
-  end.
-
-Ltac of_ap_expr :=
-  match goal with
-    | H1 : open_funcS ?e = Some (of_ap ?t ?u) |- _ =>
-      match goal with
-        | _ : ExprDsimul.ExprDenote.exprD' _ _ 
-              (typ2 (typ2 tyStack (typ2 t u))
-                (typ2 (typ2 tyStack t) (typ2 tyStack u))) e =
-          Some (fun _ _ => apD t u) |- _ => fail 1
-        | _ : ExprDsimul.ExprDenote.funcAs e 
-  			  (typ2 (typ2 tyStack (typ2 t u))
-                (typ2 (typ2 tyStack t) (typ2 tyStack u))) =
-   		  Some (apD t u) |- _ => fail 1
-		| H2 : ExprDsimul.ExprDenote.funcAs e 
-			   (typ2 (typ2 tyStack (typ2 t u))
-                (typ2 (typ2 tyStack t) (typ2 tyStack u))) = Some _ |- _ =>
-	 	  let H := fresh "H" in pose proof(of_ap_func_eq _ H1 H2); subst
-		| H2 : ExprDsimul.ExprDenote.exprD' _ _ 
-			   (typ2 (typ2 tyStack (typ2 t u))
-                (typ2 (typ2 tyStack t) (typ2 tyStack u))) e = Some _ |- _ =>
-	  	  let H := fresh "H" in pose proof(of_ap_eq _ H1 H2); subst
-	 end
-  end.
-
-Ltac of_stack_get_type :=
-  match goal with
-    | H1 : open_funcS ?e = Some of_stack_get |- _ =>
-      match goal with
-        | _ : ExprDsimul.ExprDenote.funcAs e
-   			  (typ2 tyString (typ2 tyStack tyVal)) = Some _ |- _ => fail 1
-        | _ : ExprDsimul.ExprDenote.exprD' _ _  
-              (typ2 tyString (typ2 tyStack tyVal)) e = Some _ |- _ => fail 1
-        | H2 : ExprDsimul.ExprDenote.funcAs e _ = Some _ |- _ =>
-  	  	  let H := fresh "H" in
-	        pose proof (of_stack_get_func_type_eq _ _ H1 H2) as H; r_inj H; repeat clear_eq; subst
-	    | H2 : ExprDsimul.ExprDenote.exprD' _ _ _ e = Some _ |- _ =>
-	      let H := fresh "H" in
-	        pose proof (of_stack_get_type_eq _ _ H1 H2) as H; r_inj H; repeat clear_eq; subst
-	  end
-  end.
-
-Ltac of_stack_get_expr :=
-  match goal with
-    | H1 : open_funcS ?e = Some of_stack_get |- _ =>
-      match goal with
-        | _ : ExprDsimul.ExprDenote.exprD' _ _ 
-              (typ2 tyString (typ2 tyStack tyVal)) e =
-          Some (fun _ _ => stack_getD) |- _ => fail 1
-        | _ : ExprDsimul.ExprDenote.funcAs e 
-  			  (typ2 tyString (typ2 tyStack tyVal)) =
-   		  Some stack_getD |- _ => fail 1
-		| H2 : ExprDsimul.ExprDenote.funcAs e 
-			   (typ2 tyString (typ2 tyStack tyVal)) = Some _ |- _ =>
-	 	  let H := fresh "H" in pose proof(of_stack_get_func_eq _ H1 H2); subst
-		| H2 : ExprDsimul.ExprDenote.exprD' _ _ 
-			   (typ2 tyString (typ2 tyStack tyVal)) e = Some _ |- _ =>
-	  	  let H := fresh "H" in pose proof(of_stack_get_eq _ H1 H2); subst
-	 end
-  end.
 
 Lemma pushSubst_sound tus tvs (t : typ) (e s : expr typ func)
   (eD : exprT tus tvs (typD (tyArr tyStack t))) (sD : exprT tus tvs (typD tySubst))
@@ -776,62 +419,35 @@ Proof.
     try (simpl; eapply mkApplySubst_sound; eassumption). {
     simpl. do 2 destruct_exprs; try (simpl; eapply mkApplySubst_sound; eassumption).
     + destruct_exprs; [|simpl; eapply mkApplySubst_sound; eassumption].
+      unfold tyArr in *.
       reduce.
-      ilf_true_type.
-      destruct (il_pointwise_ilogic ilpOk _ _ Heqb).
-      ilf_true_expr.
-      erewrite mkTrue_sound; [|assumption].
-      unfold applySubstD, fun_to_typ3.
-      do 2 rewrite exprT_App_wrap.
-      unfold trueD.
-      destruct (il_pointwise_ilogic_range ilpOk _ _ Heqb).
-      rewriteD (il_pointwise_true_eq ilpOk _ _ Heqb H0 H1).
       unfold apply_subst.
-      rewrite (il_pointwise_true_eq2 ilpOk _ _ Heqb H0 H1). reflexivity.
+      reduce.
+      apply mkTrue_sound; apply H.
     + destruct_exprs; [|simpl; eapply mkApplySubst_sound; eassumption].
+      unfold tyArr in *.
       reduce.
-      ilf_false_type. 
-      destruct (il_pointwise_ilogic ilpOk _ _ Heqb).
-      ilf_false_expr. 
-      erewrite mkFalse_sound; [|assumption].
-      unfold applySubstD, fun_to_typ3.
-      do 2 rewrite exprT_App_wrap.
-      unfold falseD.
-      destruct (il_pointwise_ilogic_range ilpOk _ _ Heqb).
-      rewriteD (il_pointwise_false_eq ilpOk _ _ Heqb H0 H1).
       unfold apply_subst.
-      rewrite (il_pointwise_false_eq2 ilpOk _ _ Heqb H0 H1). reflexivity.
-    + do 2 (destruct_exprs; try (solve [simpl; eapply mkApplySubst_sound; eassumption])).
       reduce.
-      bilf_emp_type.
-      destruct (bil_pointwise_bilogic bilpOk _ _ Heqb).
-	  unfold tyArr in *.
-      bilf_emp_expr.
-      erewrite mkEmp_sound; [|assumption].
-      unfold applySubstD, fun_to_typ3.
-      do 2 rewrite exprT_App_wrap.
-      unfold empD.
-      destruct (bil_pointwise_bilogic_range bilpOk _ _ Heqb).
-      rewriteD (bil_pointwise_emp_eq bilpOk _ _ Heqb H0 H1).
+      apply mkFalse_sound; apply H.
+    + do 2 (destruct_exprs; try (solve [simpl; eapply mkApplySubst_sound; eassumption])). 
+      unfold tyArr in *. 
+      reduce.
       unfold apply_subst.
-      rewrite (bil_pointwise_emp_eq2 bilpOk _ _ Heqb H0 H1). reflexivity.
+      reduce.
+      apply mkEmp_sound; assumption.
   } {
     simpl.
     destruct_exprs; try (solve [simpl; eapply mkApplySubst_sound; eassumption]).
     + repeat destruct_exprs; try (solve [simpl; eapply mkApplySubst_sound; eassumption]).
       * unfold tyArr in *.
         reduce.
+        unfold apply_subst.
         erewrite mkConst_sound; [|eassumption].
-        unfold applySubstD, fun_to_typ3.
-        do 2 rewrite exprT_App_wrap.
-        unfold constD.
-        rewriteD exprT_App_wrap.
-        rewriteD fun_to_typ_inv.
-        reflexivity.
-      * reduce.
-        unfold tyArr in *.
-        of_stack_get_type.
-        of_stack_get_expr.
+        reduce. reflexivity.
+      * unfold tyArr in *. 
+        reduce.
+        unfold apply_subst.
 
   Lemma applySubst_sound tus tvs s x sD
     (Hs : ExprDsimul.ExprDenote.exprD' tus tvs tySubst s = Some sD) :
@@ -839,87 +455,10 @@ Proof.
     Some (exprT_App (exprT_App (fun us vs => applySubstD tyVal) (exprT_App (fun us vs => stack_getD) (fun us vs => x))) sD).
   Proof.
     unfold applySubst.
-    repeat destruct_exprs;
-    try (solve [apply mkApplySubst_sound; [assumption|
-                red_exprD_hyp; red_exprD_goal; rewrite bf_typeof_const; red_exprD_goal; rewrite funcAs_fStackGet_eq; 
-                unfold mkString; rewrite BaseFunc.mkConst_sound; rewrite stringRD; reflexivity]]).
-  reduce.
-  
-  Lemma of_trunc_subst_func_type_eq t (f : func) (df : typD t) 
-    (Ho : open_funcS f = Some of_trunc_subst) 
-    (Hf : funcAs f t = Some df) :
-    Rty t (typ2 (tyList (tyProd tyString tyExpr)) (typ2 tyString tyExpr)).
-  Proof.
-    pose proof (of_funcAsOk _ Ho) as H; rewrite H in Hf.
-    unfold funcAs in Hf. simpl in Hf. 
-    forward; inv_all; subst.
-  Qed.
-  
-
-Ltac of_trunc_subst_type :=
-  match goal with
-    | H1 : open_funcS ?e = Some of_trunc_subst |- _ =>
-      match goal with
-        | _ : ExprDsimul.ExprDenote.funcAs e
-   			  (typ2 (tyList (tyProd tyString tyExpr)) (typ2 tyString tyExpr)) = Some _ |- _ => fail 1
-        | _ : ExprDsimul.ExprDenote.exprD' _ _  
-              (typ2 (tyList (tyProd tyString tyExpr)) (typ2 tyString tyExpr)) e = Some _ |- _ => fail 1
-        | H2 : ExprDsimul.ExprDenote.funcAs e _ = Some _ |- _ =>
-  	  	  let H := fresh "H" in
-	        pose proof (of_trunc_subst_func_type_eq _ _ H1 H2) as H; r_inj H; repeat clear_eq; subst
-	  end
-  end.
-
-  Lemma of_stack_get_func_eq (f : func) 
-    (df : typD (typ2 (tyList (tyProd tyString tyExpr)) (typ2 tyString tyExpr)))
-    (Ho : open_funcS f = Some of_trunc_subst)
-    (Hf : funcAs f (typ2 (tyList (tyProd tyString tyExpr)) (typ2 tyString tyExpr)) = Some df) :
-    df = truncSubstD.
-  Proof.
-   rewrite (of_funcAsOk _ Ho) in Hf.
-   unfold funcAs in Hf; simpl in *.
-   rewrite type_cast_refl in Hf; [| apply _].
-   unfold Rcast, Relim_refl in Hf.
-   inversion Hf. reflexivity.
-  Qed.
-  
-Ltac of_trunc_subst_expr :=
-  match goal with
-    | H1 : open_funcS ?e = Some of_trunc_subst |- _ =>
-      match goal with
-        | _ : ExprDsimul.ExprDenote.exprD' _ _ 
-              (typ2 (tyList (tyProd tyString tyExpr)) (typ2 tyString tyExpr)) e =
-          Some (fun _ _ => truncSubstD) |- _ => fail 1
-        | _ : ExprDsimul.ExprDenote.funcAs e 
-  			  (typ2 (tyList (tyProd tyString tyExpr)) (typ2 tyString tyExpr)) =
-   		  Some truncSubstD |- _ => fail 1
-		| H2 : ExprDsimul.ExprDenote.funcAs e 
-			   (typ2 (tyList (tyProd tyString tyExpr)) (typ2 tyString tyExpr)) = Some _ |- _ =>
-	 	  let H := fresh "H" in pose proof(of_stack_get_func_eq _ H1 H2); subst
-		(*| H2 : ExprDsimul.ExprDenote.exprD' _ _ 
-			   (typ2 tyString (typ2 tyStack tyVal)) e = Some _ |- _ =>
-	  	  let H := fresh "H" in pose proof(of_stack_get_eq _ H1 H2); subst*)
-	 end
-  end.
-
-of_trunc_subst_type.
-of_trunc_subst_expr.
-
-  Lemma mkTruncSubst_sound (tus tvs : tenv typ) (s : expr typ func)
-    (ds : ExprI.exprT tus tvs (typD tySubstList))
-    (Hs : ExprDsimul.ExprDenote.exprD' tus tvs tySubstList s = Some ds) :
-    ExprDsimul.ExprDenote.exprD' tus tvs tySubst (mkTruncSubst s) =
-      Some (exprT_App (fun _ _ => truncSubstD) ds).
-  Proof.
-    unfold mkTruncSubst; simpl.
-    pose proof (exprD_typeof_Some _ _ _ _ _ Hs) as Hts.
-    autorewrite with exprD_rw; simpl; forward; inv_all; subst.
-    autorewrite with exprD_rw; simpl; forward; inv_all; subst.
-    pose proof of_fTruncSubstOk as Ho.
-    pose proof (of_funcAsOk _ Ho) as H3; rewrite H3.
-    unfold funcAs; simpl; rewrite type_cast_refl; [reflexivity | apply _].
-  Qed.
-
+    repeat destruct_exprs; try (solve [
+	    apply mkApplySubst_sound; [assumption|
+	    red_exprD_goal; unfold stringR, stringD; rewrite trmRD; rewrite bf_typeof_const; red_exprD_goal; rewrite funcAs_fStackGet_eq;
+	    unfold mkString; rewrite BaseFunc.mkConst_sound; reflexivity]]).
 
   Lemma applyTruncSubst_sound tus tvs x s sD 
     (Hs : ExprDsimul.ExprDenote.exprD' tus tvs tySubstList s = Some sD) :
@@ -927,10 +466,110 @@ of_trunc_subst_expr.
       Some (exprT_App (exprT_App (fun _ _ => applySubstD tyVal)
              (exprT_App (fun _ _ => stack_getD) (fun _ _ => x))) (exprT_App (fun _ _ => truncSubstD) sD)).
   Proof.
+     induction s; simpl;
+     try (solve [
+	    apply mkApplySubst_sound; [apply mkTruncSubst_sound; assumption|
+	    red_exprD_goal; unfold stringR, stringD; rewrite trmRD; rewrite bf_typeof_const; red_exprD_goal; rewrite funcAs_fStackGet_eq;
+	    unfold mkString; rewrite BaseFunc.mkConst_sound; reflexivity]]).
+     repeat destruct_exprs;
+     try (solve [
+	    apply mkApplySubst_sound; [apply mkTruncSubst_sound; assumption|
+	    red_exprD_goal; unfold stringR, stringD; rewrite trmRD; rewrite bf_typeof_const; red_exprD_goal; rewrite funcAs_fStackGet_eq;
+	    unfold mkString; rewrite BaseFunc.mkConst_sound; reflexivity]]).
+    reduce. unfold substD, substR.
+    reduce.
+    erewrite mkConst_sound; [|apply mkNull_sound].
+    reduce.
+    unfold nilD, listR. unfold apply_subst, substListD.
+    rewriteD trmDR2. reflexivity.
+     repeat destruct_exprs;
+     try (solve [
+	    apply mkApplySubst_sound; [apply mkTruncSubst_sound; assumption|
+	    red_exprD_goal; unfold stringR, stringD; rewrite trmRD; rewrite bf_typeof_const; red_exprD_goal; rewrite funcAs_fStackGet_eq;
+	    unfold mkString; rewrite BaseFunc.mkConst_sound; reflexivity]]).
+    reduce. unfold substD, consD, pairD, prodR, listR, substR, substListD.
+    reduce.
+    Check (listE (pairE eq_refl (funE (funE eq_refl eq_refl) eq_refl))).
+    rewrite Heqo13.
+    f_equal.
+    do 2 (apply functional_extensionality; intros).
+    Check trmDR2.
+    Check ((trmD
+              (trmR
+                 (trmR (t3, e3 x0 x1) (btProd tyString tyExpr)
+                  :: trmD (e0 x0 x1) (listE eq_refl)) (listE eq_refl))
+              (listE (pairE eq_refl (funE (funE eq_refl eq_refl) eq_refl))))).  
+
+                 Check ((trmR (t3, e3 x0 x1) (btProd tyString tyExpr)
+                  :: (trmD (e0 x0 x1) (listE eq_refl)))).
+                  Check @listE.
+                  Check eq_trans.
+  Lemma trmDR_cons (t : typ) A B (x : A) (xs : list A) (e1 : typD t = A) (e2 : typD t = B) :
+    (trmD (trmR (x :: xs) (listE e1)) (listE e2)) =
+      trmD (trmR x e1) e2 :: trmD (trmR xs (listE e1)) (listE e2). 
+  Proof.
+	unfold trmD, trmR, listE, eq_ind, eq_rect_r, eq_rect, eq_sym, id.
+	clear.
+	revert e1 e2.
+	generalize (btList t).
+	generalize dependent (typD (tyList t)).
+	generalize dependent (typD t); intros; repeat subst. reflexivity.
+  Qed.
+  
+  Lemma trmR_eq_refl A t (x : A) (e : typD t = A) :
+    trmR (trmR x e) eq_refl = trmR x e.
+  Proof.
+    unfold trmR, eq_rect_r, eq_rect, eq_sym.
+    clear.
+    revert e.
+    generalize dependent (typD t); intros; subst. reflexivity.
+  Qed.
+  
+  rewrite trmDR_cons.
+  
+  rewrite trmR_eq_refl.
+
+  Lemma prodDR (t u : typ) A B C D (x : A) (y : B) (e1 : typD t = A) (e2 : typD u = B) (e3 : typD t = C) (e4 : typD u = D) :
+    trmD (trmR (x, y) (pairE e1 e2)) (pairE e3 e4) = 
+    (trmD (trmR x e1) e3, trmD (trmR y e2) e4).
+  Proof.
+    unfold trmD, trmR, pairE, eq_ind, eq_rect_r, eq_rect, eq_sym, id.
+    clear.
+    revert e1 e2 e3 e4.
+    generalize (btProd t u).
+    generalize dependent (tyProd t u).
+    generalize dependent (typD t).
+    generalize dependent (typD u).
+    do 3 intros.
+    generalize dependent (typD t0).
+    intros; repeat subst. reflexivity.
+  Qed.
+  
+  replace (pairE (t := tyString) (u := tyExpr) eq_refl eq_refl) with (btProd tyString tyExpr). 
+  
+  rewriteD prodDR.
+  
+  
+  
+  
+  rewriteD trmDR2.
+  Opaque pairE.
+  unfold eq_sym, eq_trans, funE. simpl.
+  simpl.
+  
+  rewriteD trmD_cons.
+    unfold listE, pairE.
+    rewriteD trmDR2.
+    erewrite mkApplySubst_sound.
+    Focus 2.
+    apply mkTruncSubst_sound.
+    reduce.
+    reflexivity.
     induction s; simpl;
     try (solve [apply mkApplySubst_sound; [apply mkTruncSubst_sound; assumption |
                 red_exprD_hyp; red_exprD_goal; rewrite bf_typeof_const; red_exprD_goal; rewrite funcAs_fStackGet_eq; 
                 unfold mkString; rewrite BaseFunc.mkConst_sound; rewrite stringRD; reflexivity]]).
+    Focus 2.
     + repeat (destruct_exprs;
       try (solve [apply mkApplySubst_sound; [apply mkTruncSubst_sound; assumption |
                 red_exprD_hyp; red_exprD_goal; rewrite bf_typeof_const; red_exprD_goal; rewrite funcAs_fStackGet_eq; 
@@ -938,7 +577,61 @@ of_trunc_subst_expr.
       reduce.
 
 repeat rewrite exprT_App_wrap_sym.
-unfold applySubstD, truncSubstD, stack_getD, fun_to_typ3, fun_to_typ2.
+repeat rewrite exprT_App_wrap_tyArrD.
+repeat unfold applySubstD, truncSubstD, substR, substD, stack_getD, tyArrR3, tyArrD2, tyArrD2', tyArrR2, tyArrR3', tyArrR2', tyArrR, tyArrR', tyArrD, tyArrD'.
+repeat rewrite trmDR.
+Check @trmDR.
+repeat rewriteD @trmDR.
+unfold substListD, nilD.
+unfold listR.
+Check @listE.
+Check @trmR.
+Check (trmD (trmR nil (listE eq_refl))
+              (listE (pairE eq_refl (funE (funE eq_refl eq_refl) eq_refl)))).
+
+
+
+rewrite trmDR2.
+
+erewrite mkConst_sound; [|eapply mkNull_sound].
+rewrite exprT_App_wrap_tyArrD.
+unfold tyArrD, tyArrD', constD, tyArrR, tyArrR'.
+rewrite trmDR. reflexivity.
+
+
+Focus 2. intros; subst.
+reflexivity.
+pose proof (@trmDR2 tyList list (@listE typ _ _ _)).
+rewriteD H.
+rewriteD trmDR2.
+
+pose proof (@trmDR2 tyList list (tyProd tyString (tyArr tyStack tyExpr)) (String.string * (@Open.expr (typD tyString) (typD tyVal))) (@listE typ _ _ _) nil (pairE eq_refl (funE (funE eq_refl eq_refl) eq_refl))).
+unfold listE.
+simpl.
+rewriteD @trmDR2.
+  generalize dependent (typD (f t)).
+  generalize dependent (typD t).
+  intros; subst.
+  generalize (f t).
+  generalize dependent (typD (f t)).
+rewriteD @trmDR.
+simpl.
+
+erewrite mkConst_sound; [|eapply mkNull_sound].
+f_equal. rewrite exprT_App_wrap_tyArrD.
+do 2 (apply functional_extensionality; intros).
+simpl.
+
+rewriteD @trmDR.
+Print ap.
+rewrite mkConst_sound.
+assert (tyExpr = tyVal) by admit.
+rewrite H.
+Check mkNull_sound.
+rewrite mkNull_sound.
+rewrite trmDR.
+unfold 
+unfold substD.
 repeat rewriteD fun_to_typ_inv.
 Lemma substDR s : substD (substR s) = s.
 Proof.
